
\subsection*{Worked Proof}

%%%Insert this to get the typewriter font so it looks like a real movie script
{\ttfamily
\fontdimen2\font=0.4em
\fontdimen3\font=0.2em
\fontdimen4\font=0.1em
\fontdimen7\font=0.1em
\hyphenchar\font=`\-

% Change to remove ordered and pick last non-0 coord c_j and note that j > 1
\hypertarget{scripts_linear_independence_thm}{Here we will work through a quick version of the proof of} Theorem~\ref{linear_dependence}. Let $\{ v_i \}$ denote a set of linearly dependent vectors, so $\sum_i c^i v_i = 0$ where there exists some $c^k \neq 0$. Now without loss of generality we order our vectors such that $c^1 \neq 0$, and we can do so since addition is commutative (i.e. $a + b = b + a$). Therefore we have
\begin{align*}
c^1 v_1 & = -\sum_{i=2}^n c^i v_i
\\ v_1 & = -\sum_{i=2}^n \frac{c^i}{c^1} v_i
\end{align*}
and we note that this argument is completely reversible since every $c^i \neq 0$ is invertible and $0 / c^i = 0$.

} % Closing bracket for font

%\newpage
